Reformalizing semantics

src/automata.v
@@ -1,4 +1,10 @@
-Require Import 
+(***********************************************)
+(*   Small library to manipulate DFAs in Coq   *)
+(*            Arthur Correnson                 *)
+(*      <arthur.correnson@ens-rennes.fr>       *)
+(***********************************************)
+
+Require Import
   Lists.List
   Init.Nat
   Lia
@@ -9,238 +15,122 @@ Import ListNotations.
 
 Set Implicit Arguments.
 
+(***********************************************)
+(** * Definitions                              *)
+(***********************************************)
+
+
+(** Definition of DFAs *)
 Record dfa (S A : Type) := DFA {
   initial_state : S;
   is_final : S -> bool;
   next : S -> A -> S
 }.
 
-Definition sem_denot_dfa (S A : Type) (w : list A) (m : dfa S A) : bool :=
-  is_final m (fold_left (next m) w (initial_state m)).
+(** Run a DFA [m] from state [q] *)
+Definition run_from (S A : Type) (m : dfa S A) (q : S) (w : list A) : S :=
+  fold_left (next m) w q.
 
-(* Inductive sem_op_dfa (S A : Type) (m : dfa S A) : S -> A -> S -> Prop :=
-  | step : forall q c,
-    sem_op_dfa m q c (next m q c). *)
+(**
+  Check if a word [w] is accepted by a dfa [m].
+  [accept m] can be thought of as [m]'s denotational semantic.
+*)
+Definition accept (S A : Type) (m : dfa S A) (w : list A) : bool :=
+  is_final m (run_from m (initial_state m) w).
 
-Inductive sem_op_dfa (S A : Type) (m : dfa S A) : S -> list A -> S -> Prop :=
-  | no_step   : forall q,
-    sem_op_dfa m q [] q
+(**
+  Inductive predicate indicating the existence of a path ([q] [w] [q']) wrt [m].
+  Usefull for proofs requiring to keep track of the states
+  taken by the dfa.
+  [path m] can be thought of as [m]'s operational semantic.
+*)
+Inductive path (S A : Type) (m : dfa S A) : S -> list A -> S -> Prop :=
+  (* Epsilon transitions can always be simulated *)
+  | epsilon_path : forall q,
+    path m q [] q
   
-  | one_step  : forall q c,
-    sem_op_dfa m q [c] (next m q c)
+  (* There exists a path of size 1 ([q] [c] [q']) for every transition (q, c, q') *)
+  | unit_path  : forall q c,
+    path m q [c] (next m q c)
   
-  | steps     : forall q q' c w,
-    sem_op_dfa m (next m q c) w q' ->
-    sem_op_dfa m q (c::w) q'.
-  
-Lemma steps_r :
-  forall S A (m : dfa S A) q q' c w,
-    sem_op_dfa m q w  q' ->
-    sem_op_dfa m q (w ++ [c]) (next m q' c).
+  (* If there exists a path ([q] [w] [q']) and a path ([q'] [w'] [q''])
+    then, there exists a path ([q] [w.w'] [q'']) *)
+  | trans_path : forall q1 q2 q3 w1 w2,
+    path m q1 w1 q2 ->
+    path m q2 w2 q3 ->
+    path m q1 (w1 ++ w2) q3.
+
+
+(***********************************************)
+(** * Usefull properties                       *)
+(***********************************************)
+
+(**
+  If there exists a path ([q'] [w] [q'']) and if
+  (q, a, q') is a transition, then there exists
+  a path ([q] [a.w] [q''])
+*)
+Lemma cons_path:
+  forall (S A : Type) (m : dfa S A) a w q1 q2,
+  path m (next m q1 a) w q2 ->
+  path m q1 (a::w) q2.
 Proof.
   intros.
-  dependent induction H; simpl.
-  - apply one_step.
-  - apply steps, one_step.
-  - apply steps.
-    apply IHsem_op_dfa.
+  dependent destruction H.
+  - apply unit_path.
+  - replace ([a; c]) with ([a] ++ [c]) by reflexivity.
+    eapply trans_path; apply unit_path.
+  - replace (a :: w1 ++ w2) with ([a] ++ w1 ++ w2) by reflexivity.
+    eapply trans_path.
+    + apply unit_path.
+    + eapply trans_path.
+      ++ apply H.
+      ++ apply H0.
 Qed.
 
-(* Notation "[| m |] w " := (sem_denot_dfa w m) (at level 40).
-Notation "[| m |] ( w , q )" := (fold_left (next m) w q) (at level 40).
-Notation "( m , q1 , w ) --> q2" := (sem_op_dfa m q1 w q2) (at level 40). *)
+Notation "( m , q1 , w ) --> q2" := (path m q1 w q2) (at level 80).
 
-
-Lemma fold_trans :
+(**
+  If runing [m] on a word [w] from state [q] places [m] 
+  in a new state [q'], then there exists a path ([q] [w] [q'])
+  and reciprocally.
+*)
+Lemma run_from_path :
   forall S A (m : dfa S A) w q1 q2,
-  fold_left (next m) w q1 = q2
+  run_from m q1 w = q2
   <->
-  sem_op_dfa m q1 w q2.
+  path m q1 w q2.
 Proof.
   intros. split.
   - dependent induction w; intros H.
-    + elim H. apply no_step.
-    + apply steps.
-      apply IHw.
-      assumption.
-  - dependent induction w; intros H.
-    + inversion H; subst; reflexivity.
-    + inversion H; subst.
-      ++ reflexivity.
-      ++ simpl. apply IHw. assumption.
+    + elim H. apply epsilon_path.
+    + apply (cons_path _ _ (IHw _ _ H)).
+  - intro.
+    dependent induction H.
+    + reflexivity.
+    + reflexivity.
+    + unfold run_from in *.
+      rewrite fold_left_app; subst.
+      reflexivity.
 Qed.
 
-
-Theorem sem_equiv :
+(**
+  If [m] accepts [w], then there exists a path from the initial state
+  to a terminal state and reciprocally.
+*)
+Theorem accept_path :
   forall S A (m : dfa S A) w,
-  sem_denot_dfa w m = true
+  accept m w = true
   <->
-  exists k, is_final m k = true /\ sem_op_dfa m (initial_state m) w k.
+  exists k, is_final m k = true /\ path m (initial_state m) w k.
 Proof.
-  intros S A m w. 
-  eelim (fold_trans m w).
-  intros. split.
-  - intro.
-    unfold sem_denot_dfa in H1.
-    exists (fold_left (next m) w (initial_state m)).
-    split; [assumption | apply H; reflexivity].
-  - intros [x [H1 H2]].
-    apply fold_trans in H2.
-    unfold sem_denot_dfa; simpl.
+  intros S A m w.
+  edestruct (run_from_path m w (initial_state m)) as [H1 H2]; split.
+  + intro H3.
+    exists (run_from m (initial_state m) w).
+    split; [exact H3 | apply H1; reflexivity].
+  + intros [qf [H3 H4]].
+    apply run_from_path in H4.
     subst.
     assumption.
 Qed.
-
-Inductive binary := I | O.
-
-Inductive states := S0 | S1 | S2.
-
-Definition m3 : dfa states binary := {|
-  initial_state := S0;
-  is_final s := match s with S0 => true | _ => false end;
-  next s x :=
-    match s, x with
-    | S0, O => S0
-    | S0, I => S1
-    | S1, O => S2
-    | S1, I => S0
-    | S2, O => S1
-    | S2, I => S1
-    end
-|}.
-
-Fixpoint base_2' (w : list binary) : nat :=
-  match w with
-  | [] => 0
-  | I::x => pow 2 (length x) + (base_2' x)
-  | O::x => base_2' x
-  end.
-
-Definition nat_of_bin n :=
-  match n with
-  | I => 1
-  | O => 0
-  end.
-
-Definition base_2 w := fold_left (fun a b => nat_of_bin b + 2 * a) w 0.
-
-Definition divide a b := exists k, b = a*k.
-
-Theorem bin_ind:
-    forall P : list binary -> Prop,
-    P [] ->
-    (forall (w : list binary), P w -> P (w ++ [I])) ->
-    (forall (w : list binary), P w -> P (w ++ [O])) ->
-    forall w, P w.
-Proof.
-Admitted.
-
-Lemma base_2_wI:
-  forall w, 
-  base_2 (w ++ [I]) = 2*(base_2 w) + 1.
-Proof.
-  induction w.
-  - simpl. reflexivity.
-  - unfold base_2.
-    rewrite fold_left_app.
-    simpl.
-    lia.
-Qed.
-
-Lemma base_2_WO:
-  forall w,
-  base_2 (w ++ [O]) = 2 *(base_2 w).
-Proof.
-  induction w.
-  - simpl; reflexivity.
-  - unfold base_2.
-    rewrite fold_left_app.
-    simpl.
-    lia.
-Qed.
-
-Lemma case_S0:
-  forall w,
-  sem_op_dfa m3 S0 w S0 ->
-  divide 3 (base_2 w).
-Proof.
-  intro.
-  elim w using bin_ind.
-  + intro; exists 0; reflexivity.
-  + intros.
-    inversion H0; subst.
-    ++ assert (forall w, [] <> w ++ [I]).
-      * intro. induction w1; discriminate.
-      * apply H1 in H3. contradiction.
-    ++ 
-Abort.
-
-
-(* Lemma trans_S0_I :
-  forall w,
-  sem_op_dfa m3 S0 w S0 ->
-  sem_op_dfa m3 S0 (w ++ [I]) S1.
-Proof.
-  intros.
-  replace (S1) with (next m3 S0 I) by reflexivity.
-  apply steps_r.
-  assumption.
-Qed.
-
-Lemma trans_S0_O :
-  forall w,
-  sem_op_dfa m3 S0 w S0 ->
-  sem_op_dfa m3 S0 (w ++ [O]) S0.
-Proof.
-  intros.
-  replace (S0) with (next m3 S0 O) by reflexivity.
-  apply steps_r.
-  assumption.
-Qed.
-
-Lemma trans_S1_I: 
-  forall w,
-  sem_op_dfa m3 S0 w S1 ->
-  sem_op_dfa m3 S0 (w ++ [I]) S2.
-Proof.
-  intros.
-  replace (S2) with (next m3 S1 I) by reflexivity.
-  apply steps_r.
-  assumption.
-Qed.
- *)
-
-Lemma sem_app:
-  forall S A (m : dfa S A) q1 q2 q3 w1 w2,
-  sem_op_dfa m q1 w1 q2 ->
-  sem_op_dfa m q2 w2 q3 ->
-  sem_op_dfa m q1 (w1 ++ w2) q3.
-Proof.
-  intros.
-  dependent induction H0.
-  - rewrite app_nil_r. assumption.
-  - apply steps_r. assumption.
-  - dependent induction H.
-    + simpl.
-      apply steps. assumption.
-    + simpl. apply steps.
-      apply steps.
-      assumption.
-    + simpl.
-      apply steps.
-      apply IHsem_op_dfa.
-      ++ assumption.
-      ++ intro.
-
-Qed.
-
-Lemma m3_correct:
-  forall w, 
-  sem_op_dfa m3 S0 w S0 ->
-  divide 3 (base_2 w).
-Proof.
-  intro.
-  elim w using bin_ind.
-  + intro.
-    exists 0; reflexivity.
-  + intros.
